## Purpose

We want to caluculate how $v_\parallel$ and $v_\perp$ intaract each other under **acclelation** and **mirror force** process.

---

## Situation

---

### Resonance

Some ion accelarated by something(like resonance). 

We imagine ion cycltron resonance.

For example, ion is accelareted by ion cylotron waves.

**Resonance condition**

$\Omega_i = \omega - k_\parallel v_\parallel$

Under this condition, ion is accelarated.

**Assumption**
- Wave is electrostatic
    - $B_1 = 0$

- Wave accelate only $v_\perp$ under ion cylctron resonance.
    - That's mean, $\frac{dv_\perp}{dt} = E\frac{q}{m}$
    - And, not accelate $v_\parallel$
    - Now, $E$ is constant

---

### Mirror force

$m\frac{dv_\parallel}{dt} = \mu \nabla_\parallel B$

**Assumption**
- Dipole magetic filed

---
## Resonance limitation

**Assume** that there are only waves with frequencies close to $\Omega_i$.
- Why?
    - Because, An upper limit to the acceleration of ions is seen by observation.
    - Waves of various frequency bands, especially those lower than $\Omega_i$, should accelerate the ions to a significant degree.

(Note : $\Omega_i = \omega - k_\parallel v_\parallel$)

Based on this assumption, the resonant ions, when accelerated **by the mirror force**, should leave the resonance condition and **no longer accelerate $v_\perp$**.

The magnitude of the mirror force depends on $v_\perp$. In other words, there is a nonlinear process.

â†’ We need simulation.

---

## Frame

$v_\perp$ is accelarated by $E$ (resonance).

Sometime, is not acclerated because $v_\parallel$ is over some value.

Because of mirror force, $v_\parallel$ decrease.

$v_\parallel$ is accelrated by mirror force.

---

## Equation

Mirror force does not give energy to systems.

So,  

$W = W_\parallel + W_\perp$ 

$\frac{dW_\parallel}{dt} + \frac{d W_\perp}{dt} = \frac{dW}{dt} = qE v_\perp$


$\frac{dW_\parallel}{dt} + \frac{d W_\perp}{dt} = qE v_\perp$

$\frac{1}{2}m \{\frac{d(v_\perp)^2}{dt} + \frac{d(v_\parallel)^2}{dt}\} = qE v_\perp $


$m \{v_\perp\frac{dv_\perp}{dt} + v_\parallel\frac{d v_\parallel}{dt}\} = qE v_\perp $

if $v_\perp \neq 0$, 


$\frac{dv_\perp}{dt} = \frac{qE}{m} - \frac{v_\parallel}{v_\perp}\frac{d v_\parallel}{dt} $

Mirror Force is...

$m\frac{dv_\parallel}{dt} = \mu \nabla_\parallel B$


$m\frac{dv_\parallel}{dt} = \frac{1}{2B}m v_\perp \nabla_\parallel B$


$\frac{dv_\parallel}{dt} = v_\perp^2\frac{1}{2}  \frac{1}{R_EL}\frac{3\sin\lambda(5\sin^2\lambda^2+3)}{\cos^{2}\lambda(1+3\sin^2\lambda)^{\frac{3}{2}}}$ 

$\lambda$ : Invarialnt latitude

$L$ : L-shell

$R_E$ : Earth Radius

---

## Last equations

$\frac{dv_\perp}{dt} = \frac{qE}{m} - \frac{v_\parallel}{v_\perp}\frac{d v_\parallel}{dt} $

$\frac{dv_\parallel}{dt} = v_\perp^2\frac{1}{2}  \frac{1}{R_EL}\frac{3\sin\lambda(5\sin^2\lambda^2+3)}{\cos^{2}\lambda(1+3\sin^2\lambda)^{\frac{3}{2}}}$ 



---
## Appendix Grad-B

In dipole,

$B = \frac{\mu_0 M_E}{4\pi}\frac{1}{R_E^3L^3}\frac{(1+3\sin^2\lambda)^\frac{1}{2}}{\cos^6\lambda}$

$\lambda$ : Invarialnt latitude

$L$ : L-shell

$R_E$ : Earth Radius

(from Basic Space Plasma Physics)

$\nabla_\parallel B = \frac{dB}{ds} = \frac{d\lambda}{ds}\frac{dB}{d\lambda} =(\frac{ds}{d\lambda})^{-1}\frac{dB}{d\lambda} $..?

$\frac{ds}{d\lambda} = LR_E\cos\lambda(1+3\sin^2\lambda)^{\frac{1}{2}}$
(from Basic Space Plasma Physics)

$\frac{dB}{d\lambda} = \frac{\mu_0 M_E}{4\pi}\frac{1}{R_E^3L^3}\frac{\cos^6\lambda(1+3\sin^2\lambda)^\frac{-1}{2}(\frac{1}{2}6.0\sin\lambda\cos\lambda)-(1+3\sin^2\lambda)^\frac{1}{2}*6\cos^5\lambda(-\sin(\lambda))}{\cos^{12}\lambda}$
$= \frac{\mu_0 M_E}{4\pi}\frac{1}{R_E^3L^3}\frac{\cos^2\lambda(1+3\sin^2\lambda)^\frac{-1}{2}(3\sin\lambda)-(1+3\sin^2\lambda)^\frac{1}{2}*6(-\sin(\lambda))}{\cos^{7}\lambda}$


$\nabla_\parallel B = (\frac{ds}{d\lambda})^{-1}\frac{dB}{d\lambda} $

$= \frac{1}{LR_E\cos\lambda(1+3\sin^2\lambda)^{\frac{1}{2}}} \frac{\mu_0 M_E}{4\pi}\frac{1}{R_E^3L^3}\frac{\cos^2\lambda(1+3\sin^2\lambda)^\frac{-1}{2}(3.0\sin\lambda)-(1+3\sin^2\lambda)^\frac{1}{2}*6(-\sin(\lambda))}{\cos^{7}\lambda}$


$= \frac{\mu_0 M_E}{4\pi}\frac{1}{R_E^3L^3(R_EL)}\frac{\cos^2\lambda(3\sin\lambda)-(1+3\sin^2\lambda)*6(-\sin(\lambda))}{\cos^{8}\lambda(1+3\sin^2\lambda)}$


$= \frac{\mu_0 M_E}{4\pi}\frac{1}{R_E^3L^3(R_EL)}\frac{\sin\lambda(3\cos^2\lambda+6(1+3\sin^2\lambda))}{\cos^{8}\lambda(1+3\sin^2\lambda)}$


$= \frac{\mu_0 M_E}{4\pi}\frac{1}{R_E^3L^3(R_EL)}\frac{3\sin\lambda(\cos^2\lambda+2(1+3\sin^2\lambda))}{\cos^{8}\lambda(1+3\sin^2\lambda)}$


$= \frac{\mu_0 M_E}{4\pi}\frac{1}{R_E^3L^3(R_EL)}\frac{3\sin\lambda(5\sin^2\lambda^2+3)}{\cos^{8}\lambda(1+3\sin^2\lambda)}$



$\frac{\nabla_\parallel B}{B}$

$= \frac{\mu_0 M_E}{4\pi}\frac{1}{R_E^3L^3(R_EL)}\frac{3\sin\lambda(5\sin^2\lambda^2+3)}{\cos^{8}\lambda(1+3\sin^2\lambda)} \frac{4\pi}{\mu_0 M_E}R_E^3L^3
 \frac{\cos^6\lambda}{(1+3\sin^2\lambda)^\frac{1}{2}}$


$=\frac{1}{R_EL}\frac{3\sin\lambda(5\sin^2\lambda^2+3)}{\cos^{2}\lambda(1+3\sin^2\lambda)^{\frac{3}{2}}}$ 
